coq/Corps/Types.v
@@ -29,9 +29,9 @@ Section CorpsTypes.
     | UnitTyping (Γ : Ctxt) : Typed Γ uu UnitT
     | AtTyping {Γ : Ctxt} {e : expr} {τ : type} (p : PName) (pf : Typed (LockExt Γ p) e τ)
       : Typed Γ (atE p e) (AtT p τ)
-    | LetTyping {Γ : Ctxt} {e1 e2 : expr} {τ σ : type} {p : PName}
-        (pf1 : Typed Γ e1 (AtT p τ)) (pf2 : Typed (VarExt Γ p τ) e2 σ)
-      : Typed Γ (letAt p e1 e2) σ
+    | LetTyping {Γ : Ctxt} {e1 e2 : expr} {τ1 τ2 : type} {p : PName}
+        (pf1 : Typed Γ e1 (AtT p τ1)) (pf2 : Typed (VarExt Γ p τ1) e2 τ2)
+      : Typed Γ (letAt p e1 e2) τ2
     | PairTyping {Γ : Ctxt} {e1 e2 : expr} {τ1 τ2 : type}
         (pf1 : Typed Γ e1 τ1) (pf2 : Typed Γ e2 τ2)
       : Typed Γ (pair e1 e2) (TimesT τ1 τ2)
@@ -47,11 +47,11 @@ Section CorpsTypes.
     | InrTyping {Γ : Ctxt} {e : expr} {τ1 τ2 : type}
         (pf : Typed Γ e τ2)
       : Typed Γ (inr e) (PlusT τ1 τ2)
-    | CaseTyping {Γ : Ctxt} {e1 e2 e3 : expr} {τ1 τ2 σ : type}
+    | CaseTyping {Γ : Ctxt} {e1 e2 e3 : expr} {τ1 τ2 τ3 : type}
         (pf1 : Typed Γ e1 (PlusT τ1 τ2))
-        (pf2 : Typed (VarExt Γ base τ1) e2 σ)
-        (pf3 : Typed (VarExt Γ base τ2) e3 σ)
-      : Typed Γ (caseE e1 e2 e3) σ
+        (pf2 : Typed (VarExt Γ base τ1) e2 τ3)
+        (pf3 : Typed (VarExt Γ base τ2) e3 τ3)
+      : Typed Γ (caseE e1 e2 e3) τ3
     | EfqlTyping {Γ : Ctxt} {e : expr}
         (pf : Typed Γ e VoidT) (τ : type)
       : Typed Γ (efql e) τ
@@ -62,20 +62,26 @@ Section CorpsTypes.
         (pf1 : Typed Γ e1 (ArrT τ1 τ2))
         (pf2 : Typed Γ e2 τ1)
       : Typed Γ (appE e1 e2) τ2
-    | SendTyping {Γ Δ : Ctxt} {m : mod} {p q : PName} {e : expr} {τ : type}
+    | SendTyping {Γ Δ : Ctxt} {m : mod} {p q : PName} {e : expr} {τ : type} {n : nat}
         (eq : change_lock_after Γ m p q = Some Δ)
         (pf : Typed Δ e τ)
         (cs : CanSend (cons m p) (cons m q))
+        (clsd : closed_below e n)
+        (eq' : lock_location Γ (cons m p) = Some n)
       : Typed Γ (send e m p q) τ
-    | UpTyping {Γ Δ : Ctxt} {m : mod} {p : PName} {e : expr} {τ : type}
+    | UpTyping {Γ Δ : Ctxt} {m : mod} {p : PName} {e : expr} {τ : type} {n : nat}
         (eq : remove_lock_after Γ m p = Some Δ)
         (pf : Typed Δ e τ)
         (cs : CanUp m (cons m p))
+        (clsd : closed_below e n)
+        (eq' : lock_location Γ (cons m p) = Some n)
       : Typed Γ (up e m p) τ
-    | DownTyping {Γ Δ : Ctxt} {m : mod} {p : PName} {e : expr} {τ : type}
+    | DownTyping {Γ Δ : Ctxt} {m : mod} {p : PName} {e : expr} {τ : type} {n : nat}
         (eq : add_lock_after Γ m p = Some Δ)
         (pf : Typed Δ e τ)
         (cs : CanDown (cons m p) m)
+        (clsd : closed_below e n)
+        (eq' : lock_location Γ m = Some n)
       : Typed Γ (down e m p) τ
     .
 
@@ -92,18 +98,21 @@ Section CorpsTypes.
       - pose proof (change_lock_after_prefix eq) as pfx.
         rewrite (all_locks_proper eqv) in pfx.
         destruct (@change_lock_after_defined _ _ Δ m p q pfx) as [E eqE].
-        apply @SendTyping with (Δ := E); auto. apply IHtyp; auto.
+        apply @SendTyping with (Δ := E) (n := n); auto. apply IHtyp; auto.
         apply (change_lock_equiv eqv eq eqE).
+        rewrite <- (lock_location_proper (cons m p) eqv); assumption.
       - pose proof (remove_lock_after_prefix eq) as pfx.
         rewrite (all_locks_proper eqv) in pfx.
         destruct (remove_lock_after_defined pfx) as [E eqE].
-        apply @UpTyping with (Δ := E); auto. apply IHtyp; auto.
+        apply @UpTyping with (Δ := E) (n := n); auto. apply IHtyp; auto.
         apply (remove_lock_equiv eqv eq eqE).
+        rewrite <- (lock_location_proper (cons m p) eqv); assumption.
       - pose proof (add_lock_after_prefix eq) as pfx.
         rewrite (all_locks_proper eqv) in pfx.
         destruct (@add_lock_after_defined _ _ Δ m p pfx) as [E eqE].
-        apply @DownTyping with (Δ := E); auto. apply IHtyp; auto.
+        apply @DownTyping with (Δ := E) (n := n); auto. apply IHtyp; auto.
         apply (add_lock_equiv eqv eq eqE).
+        rewrite <- (lock_location_proper m eqv); assumption.
     Qed.
 
     Theorem Typed_proper : forall Γ Δ, ctxt_equiv Γ Δ -> forall e τ, Typed Γ e τ <-> Typed Δ e τ.
@@ -111,27 +120,16 @@ Section CorpsTypes.
       intros Γ Δ H0 e τ; split; intro H1; [| symmetry in H0]; eapply Typed_proper'; eassumption.
     Qed.
 
-
-    Lemma Inctxt_leq : forall {Γ Δ : Ctxt} {ξ : renaming} (lq : ctxt_leq Γ ξ Δ),
-      forall n m1 τ m2, InCtxt n m1 τ m2 Γ -> InCtxt (ξ n) m1 τ m2 Δ.
+    Lemma Typed_closed_above : forall {Γ : Ctxt} {e : expr} {τ : type},
+        Typed Γ e τ ->
+        closed_above e (num_vars Γ).
     Proof using.
-      intros Γ Δ ξ lq; induction lq; try rename τ into τ'; try rename m1 into m1'; try rename m2 into m2'; intros n m1 τ m2 i; cbn; try rewrite H0; try (inversion i; subst; constructor; auto; fail).
-      - inversion i; subst. rewrite H0; repeat (constructor; auto).
-        inversion i0; subst. rewrite H1; constructor; auto.
-        rewrite H2; repeat constructor; auto.
-      - inversion i; subst.
-        inversion i0; subst.
-        rewrite mod_app_assoc. constructor; auto.
-      - inversion i; subst.
-        rewrite <- mod_app_assoc. repeat constructor; auto.
-      - assert (m2 = mod_app m2 base) as H1 by reflexivity.
-        rewrite H1; constructor; auto.
-      - assert (m2 = mod_app m2 base) as H1 by reflexivity.
-        rewrite H1 in i. inversion i; subst.
-        cbn in *; subst. assumption.
-      - apply IHlq1 in i. apply IHlq2 in i. exact i.
+      intros Γ e τ typ; induction typ; cbn; try (econstructor; eauto; fail).
+      - apply InCtxt_lt in i; constructor; assumption.
+      - constructor; rewrite (change_lock_after_num_vars eq); assumption.
+      - constructor; rewrite (remove_lock_after_num_vars eq); assumption.
+      - constructor; rewrite (add_lock_after_num_vars eq); assumption.
     Qed.
-
 
     Theorem weakening : forall {Γ Δ : Ctxt} {ξ : renaming} (lq : ctxt_leq Γ ξ Δ)
                           (e : expr) (τ : type),
@@ -141,105 +139,348 @@ Section CorpsTypes.
       intros Γ Δ ξ lq e τ typ; revert Δ ξ lq; induction typ; intros E ξ lq; cbn;
         try (econstructor; eauto; fail).
       - econstructor; apply (Inctxt_leq lq); exact i.
-      - constructor. specialize (IHtyp (LockExt E p) ξ (LockExtLeq'' p lq)).
+      - constructor. specialize (IHtyp (LockExt E p) ξ (LockExtLeq p lq)).
         cbn in IHtyp. assumption.
       - econstructor. apply IHtyp1; auto.
-        specialize (IHtyp2 (VarExt E p τ) (renup ξ) (VarExtLeq'' p τ (fun n => eq_refl) lq)).
+        specialize (IHtyp2 (VarExt E p τ1) (renup ξ) (VarExtLeq p τ1 (fun n => eq_refl) lq)).
         cbn in IHtyp2. assumption.
       - econstructor. apply IHtyp1; assumption.
-        specialize (IHtyp2 (VarExt E base τ1) (renup ξ) (VarExtLeq'' base τ1 (fun n => eq_refl) lq));
+        specialize (IHtyp2 (VarExt E base τ1) (renup ξ) (VarExtLeq base τ1 (fun n => eq_refl) lq));
           cbn in IHtyp2; assumption.
-        specialize (IHtyp3 (VarExt E base τ2) (renup ξ) (VarExtLeq'' base τ2 (fun n => eq_refl) lq));
+        specialize (IHtyp3 (VarExt E base τ2) (renup ξ) (VarExtLeq base τ2 (fun n => eq_refl) lq));
           cbn in IHtyp3; assumption.
       - constructor;
-          specialize (IHtyp (VarExt E base τ1) (renup ξ) (VarExtLeq'' base τ1 (fun n => eq_refl) lq));
+          specialize (IHtyp (VarExt E base τ1) (renup ξ) (VarExtLeq base τ1 (fun n => eq_refl) lq));
           cbn in IHtyp; assumption.
       - pose proof (change_lock_after_prefix eq).
         rewrite (ctxt_leq_all_locks lq) in H0.
-        destruct (@change_lock_after_defined PName _ E m p q H0) as [Δ' eq'].
-        apply @SendTyping with (Δ := Δ'); auto.
-        pose proof (ctxt_leq_change_lock_after lq eq eq').
+        destruct (@change_lock_after_defined PName _ E m p q H0) as [Δ' eq''].
+        pose proof (lock_location_prefix eq') as pfx.
+        rewrite (ctxt_leq_all_locks lq) in pfx.
+        destruct (lock_location_Some pfx) as [n' eqn'].
+        apply @SendTyping with (n := n') (Δ := Δ'); auto.
+        pose proof (ctxt_leq_change_lock_after lq eq eq'').
         apply IHtyp; auto.
+        eapply closed_below_ren; eauto.
+        intros n0 H1. eapply ctxt_leq_below_lock''; eauto.
       - pose proof (remove_lock_after_prefix eq).
         rewrite (ctxt_leq_all_locks lq) in H0.
-        destruct (remove_lock_after_defined H0) as [Δ' eq'].
-        apply @UpTyping with (Δ := Δ'); auto.
-        pose proof (ctxt_leq_remove_lock_after lq eq eq').
+        destruct (lock_location_Some H0) as [n' eqn'].
+        destruct (remove_lock_after_defined H0) as [Δ' eq''].
+        apply @UpTyping with (Δ := Δ') (n := n'); auto.
+        pose proof (ctxt_leq_remove_lock_after lq eq eq'').
         apply IHtyp; auto.
+        eapply closed_below_ren; eauto.
+        intros n0 H1; eapply ctxt_leq_below_lock''; eauto.
       - pose proof (add_lock_after_prefix eq).
         rewrite (ctxt_leq_all_locks lq) in H0.
-        destruct (@add_lock_after_defined _ _ E m p H0) as [Δ' eq'].
-        apply @DownTyping with (Δ := Δ'); auto.
-        pose proof (ctxt_leq_add_lock_after lq eq eq').
+        destruct (lock_location_Some H0) as [n' eqn'].
+        destruct (@add_lock_after_defined PName H E m p H0) as [Δ' eq''].
+        apply @DownTyping with (Δ := Δ') (n := n'); auto.
+        pose proof (ctxt_leq_add_lock_after lq eq eq'').
         apply IHtyp; auto.
+        eapply closed_below_ren; eauto.
+        intros n0 H1; eapply ctxt_leq_below_lock''; eauto.
     Qed.
         
   End TypeSystem.
 
-  (* Section Substitution. *)
+  Section Substitution.
 
-  (*   Definition TypedSubst (Γ : Ctxt) (σ : substitution) (Δ : Ctxt) := *)
-  (*     all_locks Γ = all_locks Δ /\ *)
-  (*     forall x m, *)
-  (*       mod_app m (locks Γ x) = fst (vars Γ x) ->  *)
-  (*       Typed (add_lock Δ m) (σ x) (snd (vars Γ x)). *)
+    Definition add_to_subst (σ : substitution) (e : expr) : substitution :=
+      fun n => match n with
+            | 0 => e
+            | (S n) => σ n
+            end.
 
-  (*   Lemma id_subst_typed: forall Γ, TypedSubst Γ (fun x => var x) Γ. *)
-  (*   Proof using. *)
-  (*     intros Γ; split; [reflexivity | intros x m eq]. *)
-  (*     apply VarTyping with (m := fst (vars Γ x)); cbn; auto. *)
-  (*     apply surjective_pairing. *)
-  (*   Qed.       *)
+    Inductive TypedSubst : Ctxt -> substitution -> Ctxt -> Prop :=
+    | EmptySubst (σ : substitution) (Γ Δ : Ctxt) :
+      ctxt_equiv Γ EmptyCtxt -> all_locks Δ = base -> TypedSubst Γ σ Δ
+    | VarLSubst (Γ Δ : Ctxt) (m : mod) (τ : type) (e : expr) (σ1 σ2 : substitution):
+      TypedSubst Γ σ1 Δ ->
+      Typed (LockExt Δ m) e τ ->
+      (forall n, σ2 n = add_to_subst σ1 e n) ->
+      TypedSubst (VarExt Γ m τ) σ2 Δ
+    | VarRSubst (Γ Δ : Ctxt) (m : mod) (τ : type) (σ1 σ2 : substitution) :
+      TypedSubst Γ σ1 Δ ->
+      (forall n, σ2 n = ren (σ1 n) S) -> 
+      TypedSubst Γ σ2 (VarExt Δ m τ)
+    | LockSubst (Γ Δ : Ctxt) (m : mod) (σ : substitution) :
+      TypedSubst Γ σ Δ ->
+      TypedSubst (LockExt Γ m) σ (LockExt Δ m).
 
-  (*   Lemma substup_typed : forall Γ Δ σ g τ, *)
-  (*       TypedSubst Γ σ Δ -> TypedSubst (add_var Γ g τ) (substup σ) (add_var Δ g τ). *)
-  (*   Proof using. *)
-  (*     intros Γ Δ σ g τ [al_eqv typd]; split; [exact al_eqv|]; intros x m eq. *)
-  (*     destruct x; cbn in *; subst. *)
-  (*     - apply VarTyping with (m := g); cbn; reflexivity. *)
-  (*     - eapply weakening with (Δ := add_lock Δ m). *)
-  (*       split; [|split]; try (intro y); cbn; auto. *)
-  (*       apply typd; auto. *)
-  (*       Unshelve. *)
-  (*       intros n m0 H0; cbn; apply mod_app_mono_l; apply locks_mono; auto. *)
-  (*   Qed. *)
+    Theorem TypedSubstAt : forall {Γ Δ : Ctxt} {σ : substitution} {n : nat} {m1 m2 : mod} {τ : type},
+        TypedSubst Γ σ Δ ->
+        InCtxt n (mod_app m1 m2) τ m1 Γ ->
+        Typed (LockExt Δ m2) (σ n) τ.
+    Proof using.
+      intros Γ Δ σ n m1 m2 τ styp; revert n m1 m2 τ; induction styp; intros n m1 m2 τ' i.
+      - rewrite (InCtxt_proper H0) in i. dependent destruction i; cbn.
+      - dependent destruction i; cbn.
+        -- rewrite mod_base_app in H0; rewrite H1; cbn; assumption.
+        -- rewrite H1; cbn; apply IHstyp with (m1 := m0); assumption.
+      - rewrite H0. apply @weakening with (Γ := LockExt Δ m2).
+        constructor; eapply VarAddLeq; [apply ctxt_leq_refl | unfold id_renaming; auto].
+        apply IHstyp with (m1 := m1); assumption.
+      - dependent destruction i; cbn.
+        rewrite mod_app_assoc in i. apply IHstyp in i.
+        apply Typed_proper with (Δ := LockExt (LockExt Δ m) m2) in i. assumption.
+        apply LockSplitEquiv. reflexivity.
+    Qed.
 
-  (*   Theorem subst_typed : forall Γ Δ e σ τ, Typed Γ e τ -> TypedSubst Γ σ Δ -> Typed Δ (subst e σ) τ. *)
-  (*   Proof using. *)
-  (*     intros Γ Δ e σ τ typed; revert Δ σ; induction typed; try (rename σ into τ'); *)
-  (*       intros Γ'' σ typeds; cbn; *)
-  (*       try (econstructor; eauto; *)
-  (*            repeat lazymatch goal with *)
-  (*              | [ H : ?P |- ?P ] => exact H *)
-  (*              | [ IH : forall Δ σ, TypedSubst ?Γ σ Δ -> Typed Δ (subst ?e σ) ?τ, H : TypedSubst ?Γ ?σ ?Δ |- Typed ?Δ (subst ?e ?σ) ?τ ] => *)
-  (*                  exact (IH Δ σ H) *)
-  (*              | [H : TypedSubst ?Γ ?σ ?Δ |- context[add_var ?Δ ?p ?τ] ] => *)
-  (*                  lazymatch goal with *)
-  (*                  | [ _ : TypedSubst (add_var Γ p τ) (substup σ) (add_var Δ p τ) |- _ ] => fail *)
-  (*                  | _ =>  *)
-  (*                      assert (TypedSubst (add_var Γ p τ) (substup σ) (add_var Δ p τ)) by (exact (substup_typed Γ Δ σ p τ H)) *)
-  (*                  end *)
-  (*              | [ H : TypedSubst ?Γ ?σ ?Δ |- context[all_locks ?Δ]] => *)
-  (*                  lazymatch goal with *)
-  (*                  | [_ : all_locks Γ = all_locks Δ |- _ ] => fail *)
-  (*                  | _ => let eq := fresh "eq" in assert (all_locks Γ = all_locks Δ) as eq by (destruct H as [al_eqv _]; exact al_eqv); *)
-  (*                                               rewrite <- eq *)
-  (*                  end *)
-  (*         end; fail). *)
-  (*     - destruct typeds as [al_eqv typeds]. *)
-  (*       specialize (typeds n base); cbn in typeds. *)
-  (*       rewrite pf1 in typeds; cbn in typeds. *)
-  (*       rewrite mod_base_app in typeds; specialize (typeds pf2). *)
-  (*       apply type_ext with (Γ := add_lock Γ'' base); [exact typeds | symmetry; apply add_base_lock]. *)
-  (*     - apply AtTyping; apply IHtyped. *)
-  (*       destruct typeds as [al_eqv typeds]; split; [cbn; rewrite al_eqv; reflexivity|]. *)
-  (*       intros x m; cbn; intro eq. *)
-  (*       apply type_ext with (Γ := add_lock Γ'' (mod_app m p)); [|apply add_two_locks]. *)
-  (*       rewrite <- mod_app_assoc in eq. *)
-  (*       apply typeds; exact eq. *)
-  (*   Qed.                                              *)
+    Lemma TypedSubstUp : forall {Γ Δ : Ctxt} {σ : substitution} {m : mod} {τ : type},
+        TypedSubst Γ σ Δ ->
+        TypedSubst (VarExt Γ m τ) (substup σ) (VarExt Δ m τ).
+    Proof using.
+      intros Γ Δ σ m τ styp.
+      eapply VarLSubst.
+      - eapply VarRSubst; [exact styp | intro n; reflexivity].
+      - eapply VarTyping; apply @thereLockInCtxt with (m1 := base); rewrite mod_base_app; apply hereInCtxt.
+      - intro n; destruct n; cbn; reflexivity.
+    Qed.
 
-  (* End Substitution. *)
-  
+    Theorem TypeSubst_ext : forall {Γ Δ : Ctxt} {σ1 σ2 : substitution},
+        (forall n, σ1 n = σ2 n) ->
+        TypedSubst Γ σ1 Δ ->
+        TypedSubst Γ σ2 Δ.
+    Proof using.
+      intros Γ Δ σ1 σ2 ext_eq styp; revert σ2 ext_eq; induction styp; intros σ3 ext_eq;
+        try (econstructor; eauto; fail).
+      - eapply VarLSubst; eauto. intro n; rewrite <- ext_eq; auto.
+      - eapply VarRSubst; eauto. intro n; rewrite <- ext_eq; auto.
+    Qed.
+
+    Theorem TypeSubstRefl : forall {Γ : Ctxt},
+        TypedSubst Γ id_substitution Γ.
+    Proof using.
+      intro Γ; induction Γ; try (econstructor; eauto; fail).
+      econstructor; reflexivity. 
+      apply @TypeSubst_ext with (σ1 := substup id_substitution); [exact id_substup|].
+      apply TypedSubstUp. exact IHΓ.
+    Qed.
+
+    Theorem TypedSubstAllLocks : forall {Γ Δ : Ctxt} {σ : substitution},
+        TypedSubst Γ σ Δ ->
+        all_locks Γ = all_locks Δ.
+    Proof using.
+      intros Γ Δ σ typ; induction typ; cbn; auto.
+      - transitivity (@all_locks PName EmptyCtxt).
+        apply all_locks_proper; assumption.
+        cbn; symmetry; assumption.
+      - f_equal; assumption.
+    Qed.
+    
+    Theorem TypedSubstLockLocation : forall {Γ Δ : Ctxt} {σ : substitution} {i j : nat} {m : mod},
+        TypedSubst Γ σ Δ ->
+        lock_location Γ m = Some i ->
+        lock_location Δ m = Some j ->
+        forall k, i <= k -> k < num_vars Γ -> closed_below (σ k) j.
+    Proof using.
+      intros Γ Δ σ i j m styp; revert i j m; induction styp; intros i j m' eqi eqj k i_le_k k_lt_Γ;
+        cbn in *.
+      - rewrite (num_vars_proper H0) in k_lt_Γ; cbn in k_lt_Γ; inversion k_lt_Γ.
+      - destruct (lock_location Γ m') eqn: eqi'; inversion eqi; subst; clear eqi; rename eqi' into eqi.
+        rewrite H1; destruct k; [inversion i_le_k|]; cbn.
+        rewrite <- PeanoNat.Nat.succ_lt_mono in k_lt_Γ; apply le_S_n in i_le_k.
+        exact (IHstyp n j m' eqi eqj k i_le_k k_lt_Γ).
+      - destruct (lock_location Δ m') eqn:eqj'; inversion eqj; subst; clear eqj; rename eqj' into eqj.
+        rewrite H0. apply @closed_below_ren with (k' := n); [apply le_n_S|].
+        apply IHstyp with (i := i) (m := m'); assumption.
+      - rewrite <- (TypedSubstAllLocks styp) in eqj; destruct (prefixb m' (all_locks Γ)) eqn:pfx.
+        apply IHstyp with (i := i) (m := m'); assumption.
+        destruct (prefixb m' (mod_app (all_locks Γ) m)) eqn: pfx'; inversion eqi; inversion eqj; subst.
+        apply closed_below_zero.
+    Qed.
+
+    Definition unit_subst_before (σ : substitution) (n : nat) :=
+      fun m => if PeanoNat.Nat.ltb m n then @uu PName else σ m.
+
+    Lemma change_lock_after_subst : forall {Γ1 Γ2 Δ1 Δ2 : Ctxt} {σ : substitution} {m : mod} {p q : PName} {n : nat},
+        TypedSubst Γ1 σ Δ1 ->
+        change_lock_after Γ1 m p q = Some Γ2 ->
+        change_lock_after Δ1 m p q = Some Δ2 ->
+        lock_location Γ1 (cons m p) = Some n ->
+        TypedSubst Γ2 (unit_subst_before σ n) Δ2.
+    Proof using.
+      intros Γ1 Γ2 Δ1 Δ2 σ m p q n styp; revert Γ2 Δ2 m p q n; dependent induction styp;
+        intros Γ2 Δ2 n p q n' eqΓ eqΔ loc; cbn in *.
+      - eapply change_lock_after_no_locks in H1; rewrite H1 in eqΔ; inversion eqΔ.
+      - destruct (change_lock_after Γ n p q) eqn:eqΓ';
+          inversion eqΓ; subst; clear eqΓ; rename eqΓ' into eqΓ.
+        destruct (lock_location Γ (cons n p)) eqn:loc';
+          inversion loc; subst; clear loc; rename loc' into loc.
+        apply VarLSubst with (e := uu) (σ1 := unit_subst_before σ1 n0).
+        apply IHstyp with (m := n) (p := p) (q := q); auto.
+        apply UnitTyping.
+        intro n1; destruct n1; cbn. reflexivity.
+        unfold unit_subst_before.
+        destruct (PeanoNat.Nat.ltb n1 n0) eqn:eq.
+        rewrite PeanoNat.Nat.ltb_lt in eq; rewrite PeanoNat.Nat.succ_lt_mono in eq; rewrite <- PeanoNat.Nat.ltb_lt in eq;
+          rewrite eq; reflexivity.
+        destruct (PeanoNat.Nat.ltb (S n1) (S n0)) eqn:eq'.
+        rewrite PeanoNat.Nat.ltb_lt in eq'; apply <- PeanoNat.Nat.succ_lt_mono in eq'; rewrite <- PeanoNat.Nat.ltb_lt in eq';
+          rewrite eq' in eq; inversion eq.
+        rewrite H1; cbn; reflexivity.
+      - destruct (change_lock_after Δ n p q) eqn:eqΔ'; inversion eqΔ; subst; clear eqΔ; rename eqΔ' into eqΔ; rename c into Δ2.
+        apply VarRSubst with (σ1 := unit_subst_before σ1 n').
+        eapply IHstyp; eauto.
+        intro n0. unfold unit_subst_before.
+        destruct (PeanoNat.Nat.ltb n0 n'); cbn; auto.
+      - rewrite <- (TypedSubstAllLocks styp) in eqΔ.
+        destruct (prefixb (cons n p) (all_locks Γ)) eqn:pfx;
+          [| destruct (remove_Prefix (all_locks Γ) n) as [m''|]; [|inversion eqΓ]].
+        -- eapply IHstyp; eauto.
+        -- destruct (prefixb (cons m'' p) m) eqn:pfx'; inversion eqΓ; inversion eqΔ; subst; clear eqΓ eqΔ.
+           destruct (prefixb (cons n p) (mod_app (all_locks Γ) m)) eqn:pfx'';
+             inversion loc; subst; clear loc.
+           apply LockSubst. eapply TypeSubst_ext; [| exact styp].
+           intro n0. unfold unit_subst_before.
+           destruct (PeanoNat.Nat.ltb n0 0) eqn:eq; [| reflexivity].
+           rewrite PeanoNat.Nat.ltb_lt in eq; inversion eq.
+    Qed.
+
+    Lemma remove_lock_after_subst : forall {Γ1 Γ2 Δ1 Δ2 : Ctxt} {σ : substitution} {m : mod} {p : PName} {n : nat},
+        TypedSubst Γ1 σ Δ1 ->
+        remove_lock_after Γ1 m p = Some Γ2 ->
+        remove_lock_after Δ1 m p = Some Δ2 ->
+        lock_location Γ1 (cons m p) = Some n ->
+        TypedSubst Γ2 (unit_subst_before σ n) Δ2.
+    Proof using.
+      intros Γ1 Γ2 Δ1 Δ2 σ m p n styp; revert Γ2 Δ2 m p n; dependent induction styp;
+        intros Γ2 Δ2 n p n' eqΓ eqΔ loc; cbn in *.
+      - eapply remove_lock_after_no_locks in H1; rewrite H1 in eqΔ; inversion eqΔ.
+      - destruct (remove_lock_after Γ n p) eqn:eqΓ';
+          inversion eqΓ; subst; clear eqΓ; rename eqΓ' into eqΓ.
+        destruct (lock_location Γ (cons n p)) eqn:loc';
+          inversion loc; subst; clear loc; rename loc' into loc.
+        apply VarLSubst with (e := uu) (σ1 := unit_subst_before σ1 n0).
+        apply IHstyp with (m := n) (p := p); auto.
+        apply UnitTyping.
+        intro n1; destruct n1; cbn. reflexivity.
+        unfold unit_subst_before.
+        destruct (PeanoNat.Nat.ltb n1 n0) eqn:eq.
+        rewrite PeanoNat.Nat.ltb_lt in eq; rewrite PeanoNat.Nat.succ_lt_mono in eq; rewrite <- PeanoNat.Nat.ltb_lt in eq;
+          rewrite eq; reflexivity.
+        destruct (PeanoNat.Nat.ltb (S n1) (S n0)) eqn:eq'.
+        rewrite PeanoNat.Nat.ltb_lt in eq'; apply <- PeanoNat.Nat.succ_lt_mono in eq'; rewrite <- PeanoNat.Nat.ltb_lt in eq';
+          rewrite eq' in eq; inversion eq.
+        rewrite H1; cbn; reflexivity.
+      - destruct (remove_lock_after Δ n p) eqn:eqΔ'; inversion eqΔ; subst; clear eqΔ; rename eqΔ' into eqΔ; rename c into Δ2.
+        apply VarRSubst with (σ1 := unit_subst_before σ1 n').
+        eapply IHstyp; eauto.
+        intro n0. unfold unit_subst_before.
+        destruct (PeanoNat.Nat.ltb n0 n'); cbn; auto.
+      - rewrite <- (TypedSubstAllLocks styp) in eqΔ.
+        destruct (prefixb (cons n p) (all_locks Γ)) eqn:pfx;
+          [| destruct (remove_Prefix (all_locks Γ) n) as [m''|]; [|inversion eqΓ]].
+        -- eapply IHstyp; eauto.
+        -- destruct (prefixb (cons m'' p) m) eqn:pfx'; inversion eqΓ; inversion eqΔ; subst; clear eqΓ eqΔ.
+           destruct (prefixb (cons n p) (mod_app (all_locks Γ) m)) eqn:pfx'';
+             inversion loc; subst; clear loc.
+           apply LockSubst. eapply TypeSubst_ext; [| exact styp].
+           intro n0. unfold unit_subst_before.
+           destruct (PeanoNat.Nat.ltb n0 0) eqn:eq; [| reflexivity].
+           rewrite PeanoNat.Nat.ltb_lt in eq; inversion eq.
+    Qed.
+
+    Lemma add_lock_after_subst : forall {Γ1 Γ2 Δ1 Δ2 : Ctxt} {σ : substitution} {m : mod} {p : PName} {n : nat},
+        TypedSubst Γ1 σ Δ1 ->
+        add_lock_after Γ1 m p = Some Γ2 ->
+        add_lock_after Δ1 m p = Some Δ2 ->
+        lock_location Γ1 m = Some n ->
+        TypedSubst Γ2 (unit_subst_before σ n) Δ2.
+    Proof using.
+    Admitted.
+    (*         intros Γ1 Γ2 Δ1 Δ2 σ m p n styp; revert Γ2 Δ2 m p n; dependent induction styp; *)
+    (*     intros Γ2 Δ2 n p n' eqΓ eqΔ loc; cbn in *. *)
+    (*   - eapply add_lock_after_no_locks in H1; rewrite H1 in eqΔ; inversion eqΔ. *)
+    (*   - destruct (remove_lock_after Γ n p) eqn:eqΓ'; *)
+    (*       inversion eqΓ; subst; clear eqΓ; rename eqΓ' into eqΓ. *)
+    (*     destruct (lock_location Γ (cons n p)) eqn:loc'; *)
+    (*       inversion loc; subst; clear loc; rename loc' into loc. *)
+    (*     apply VarLSubst with (e := uu) (σ1 := unit_subst_before σ1 n0). *)
+    (*     apply IHstyp with (m := n) (p := p); auto. *)
+    (*     apply UnitTyping. *)
+    (*     intro n1; destruct n1; cbn. reflexivity. *)
+    (*     unfold unit_subst_before. *)
+    (*     destruct (PeanoNat.Nat.ltb n1 n0) eqn:eq. *)
+    (*     rewrite PeanoNat.Nat.ltb_lt in eq; rewrite PeanoNat.Nat.succ_lt_mono in eq; rewrite <- PeanoNat.Nat.ltb_lt in eq; *)
+    (*       rewrite eq; reflexivity. *)
+    (*     destruct (PeanoNat.Nat.ltb (S n1) (S n0)) eqn:eq'. *)
+    (*     rewrite PeanoNat.Nat.ltb_lt in eq'; apply <- PeanoNat.Nat.succ_lt_mono in eq'; rewrite <- PeanoNat.Nat.ltb_lt in eq'; *)
+    (*       rewrite eq' in eq; inversion eq. *)
+    (*     rewrite H1; cbn; reflexivity. *)
+    (*   - destruct (remove_lock_after Δ n p) eqn:eqΔ'; inversion eqΔ; subst; clear eqΔ; rename eqΔ' into eqΔ; rename c into Δ2. *)
+    (*     apply VarRSubst with (σ1 := unit_subst_before σ1 n'). *)
+    (*     eapply IHstyp; eauto. *)
+    (*     intro n0. unfold unit_subst_before. *)
+    (*     destruct (PeanoNat.Nat.ltb n0 n'); cbn; auto. *)
+    (*   - rewrite <- (TypedSubstAllLocks styp) in eqΔ. *)
+    (*     destruct (prefixb (cons n p) (all_locks Γ)) eqn:pfx; *)
+    (*       [| destruct (remove_Prefix (all_locks Γ) n) as [m''|]; [|inversion eqΓ]]. *)
+    (*     -- eapply IHstyp; eauto. *)
+    (*     -- destruct (prefixb (cons m'' p) m) eqn:pfx'; inversion eqΓ; inversion eqΔ; subst; clear eqΓ eqΔ. *)
+    (*        destruct (prefixb (cons n p) (mod_app (all_locks Γ) m)) eqn:pfx''; *)
+    (*          inversion loc; subst; clear loc. *)
+    (*        apply LockSubst. eapply TypeSubst_ext; [| exact styp]. *)
+    (*        intro n0. unfold unit_subst_before. *)
+    (*        destruct (PeanoNat.Nat.ltb n0 0) eqn:eq; [| reflexivity]. *)
+    (*        rewrite PeanoNat.Nat.ltb_lt in eq; inversion eq. *)
+    (* Qed. *)
+
+
+    Theorem TypedSubstitution : forall {Γ Δ : Ctxt} {σ : substitution} {e : expr} {τ : type},
+        Typed Γ e τ ->
+        TypedSubst Γ σ Δ ->
+        Typed Δ (subst e σ) τ.
+    Proof using.
+      intros Γ Δ σ e τ typ; revert Δ σ; induction typ; try rename Δ into Δ'; intros Δ σ styp; cbn;
+        try (econstructor; eauto; fail).
+      - apply Typed_proper with (Γ := LockExt Δ base); [constructor; reflexivity |].
+        eapply @TypedSubstAt; [exact styp| cbn; exact i].
+      - constructor.
+        apply IHtyp; constructor; auto; fail.
+      - econstructor. apply IHtyp1; auto. apply IHtyp2.
+        apply TypedSubstUp; auto.
+      - econstructor; [apply IHtyp1 | apply IHtyp2 | apply IHtyp3]; try apply TypedSubstUp; auto.
+      - constructor; apply IHtyp; apply TypedSubstUp; auto.
+      - pose proof (change_lock_after_prefix eq).
+        rewrite (TypedSubstAllLocks styp) in H0.
+        rename Δ' into Γ';
+          destruct (@change_lock_after_defined PName _ Δ m p q H0) as [Δ' eqΔ'].
+        destruct (lock_location_Some H0) as [x eqx].
+        apply @SendTyping with (n := x) (Δ := Δ'); auto.
+        rewrite (@closed_below_subst_ext PName e σ (unit_subst_before σ n) n); auto.
+        apply IHtyp. eapply change_lock_after_subst; eauto.
+        intros k n_le_k; unfold unit_subst_before; destruct (PeanoNat.Nat.ltb k n) eqn:eq'';
+          [rewrite PeanoNat.Nat.ltb_lt in eq''; lia| reflexivity].
+        apply @closed_narrow_subst with (n := 0) (m := n) (j := num_vars Γ).
+        -- intros k H1 H2;  inversion H2.
+        -- intros k H1 H2;
+             eapply @TypedSubstLockLocation with (m := (cons m p)); eauto.
+        -- rewrite (change_lock_after_num_vars eq).
+           eapply Typed_closed_above; eauto.
+        -- fold (closed_below e n); assumption.
+      - pose proof (remove_lock_after_prefix eq).
+        rewrite (TypedSubstAllLocks styp) in H0.
+        rename Δ' into Γ';
+          destruct (@remove_lock_after_defined PName _ Δ m p H0) as [Δ' eqΔ'].
+        destruct (lock_location_Some H0) as [x eqx].
+        apply @UpTyping with (n := x) (Δ := Δ'); auto.
+        rewrite (@closed_below_subst_ext PName e σ (unit_subst_before σ n) n); auto.
+        apply IHtyp. eapply remove_lock_after_subst; eauto.
+        intros k n_le_k; unfold unit_subst_before; destruct (PeanoNat.Nat.ltb k n) eqn:eq'';
+          [rewrite PeanoNat.Nat.ltb_lt in eq''; lia| reflexivity].
+        apply @closed_narrow_subst with (n := 0) (m := n) (j := num_vars Γ).
+        -- intros k H1 H2;  inversion H2.
+        -- intros k H1 H2;
+             eapply @TypedSubstLockLocation with (m := (cons m p)); eauto.
+        -- rewrite (remove_lock_after_num_vars eq).
+           eapply Typed_closed_above; eauto.
+        -- fold (closed_below e n); assumption.
+      - admit.        
+    Admitted.
+        
+  End Substitution.
 End CorpsTypes.
 
